Base.thy
@@ -4,7 +4,9 @@ begin
   
 section \<open>Time\<close>
 
-class time = wellorder + ordered_ab_group_add + zero_less_one +
+find_theorems name: "zero_le"
+
+class time = linordered_ab_group_add + zero_less_one +
   assumes dense: "x < y \<Longrightarrow> \<exists>z. x < z \<and> z < y"
   assumes non_trivial: "\<exists> x. x \<noteq> 0"
 begin
@@ -20,20 +22,5 @@ proof -
     then show ?case by blast
   qed
 qed
-
-
-lemma least_time_gt_0: "(LEAST n. n > 0) > 0"
-proof -
-  have "Ex (\<lambda>x. 0 < x)" using diff_gt_0_iff_gt non_trivial_neg by blast
-  thus ?thesis using LeastI_ex by auto
-qed
-
-lemma "0 < x \<Longrightarrow> (LEAST n. 0 < n) \<le> x" using Least_le by simp
-lemma ge_least_gt_0: "Least ((<) 0) \<le> x \<Longrightarrow> 0 < x" using least_time_gt_0 by auto
-
-
-lemma GreatestI_ex_time: "\<exists>t. P t \<Longrightarrow> P (Greatest P)"
-  using least_time_gt_0 local.dense local.not_less_Least by auto
-
 end
 end
